LLVM_DS_RBT/Delete/Combine.thy
@@ -10,6 +10,211 @@ interpretation llvm_prim_arith_setup .
 interpretation llvm_prim_setup .
 
 
+abbreviation "is_black_b x \<equiv> matches_rbt_pattern (Branch CP_B RVar RVar) x"
+abbreviation "is_red_b x \<equiv> matches_rbt_pattern (Branch CP_R RVar RVar) x"
+
+abbreviation "is_black_b_i x \<equiv> matches_rbt_pattern_i (Branch CP_B RVar RVar) x"
+abbreviation "is_red_b_i x \<equiv> matches_rbt_pattern_i (Branch CP_R RVar RVar) x"
+
+
+
+(*
+fun rbt_combine_ad where "rbt_combine_ad l r =
+(
+  if l = rbt.Empty then return r
+  else if r = rbt.Empty then return l
+  else if is_red_b l \<and> is_red_b r
+  then let c = combine (rbt.right l) (rbt.left r) in X
+  else if is_black_b l \<and> is_black_b r
+  then Y
+  else if is_red_b r
+  then Z
+  else W
+)
+"
+*)
+
+
+partial_function (M) combine ::
+  "('ki, 'v::llvm_rep) rbti \<Rightarrow> ('ki, 'v) rbti \<Rightarrow> ('ki, 'v) rbti llM" where
+  "combine l_p r_p = do {
+    if l_p = null then return r_p
+    else if r_p = null then return l_p
+    else do {
+      l \<leftarrow> ll_load l_p;
+      r \<leftarrow> ll_load r_p;
+      if rbt_node.color l = rbt_node.color r
+      then do {
+        combined_p \<leftarrow> combine (rbt_node.right l) (rbt_node.left r);
+        is_red_b \<leftarrow> is_red_b_i combined_p;
+        if is_red_b = ll_True then
+        do {
+            combined \<leftarrow> ll_load combined_p;
+            case combined of (RBT_NODE cc cl ck cv cr) \<Rightarrow>
+            do {
+              set_right_p cl l_p;
+              set_left_p cr r_p;
+              ll_store (RBT_NODE cc l_p ck cv r_p) combined_p;
+              return combined_p
+            }
+        }
+        else do {
+          set_left_p combined_p r_p;
+          if rbt_node.color l = 0
+          then do {
+            set_right_p r_p l_p;
+            return l_p
+          }
+          else do {
+            case l of (RBT_NODE _ ll lk lv _) \<Rightarrow>
+            do {
+              ll_free l_p;
+              balance_left ll lk lv r_p
+            }
+          }
+        }
+      }
+      else if (rbt_node.color r = 0)
+      then do {
+        combined_p \<leftarrow> combine l_p (rbt_node.left r);
+        set_left_p combined_p r_p;
+        return r_p
+      }
+      else do { 
+        combined_p \<leftarrow> combine (rbt_node.right l) r_p;
+        set_right_p combined_p l_p;
+        return l_p
+      }
+    }
+  }"
+
+
+lemma combine_correct:
+"
+  llvm_htriple
+  (\<upharpoonleft>rbt_assn l li ** \<upharpoonleft>rbt_assn r ri)
+  (combine li ri)
+  (\<lambda>x. \<upharpoonleft>rbt_assn (rbt_combine l r) x)
+"
+proof(induction l r arbitrary: li ri rule: combine.induct)
+  case (1 x)
+  then show ?case 
+    apply (subst combine.simps)
+    apply vcg
+    done
+next
+  case (2 v va vb vc vd)
+  then show ?case 
+    apply (subst combine.simps)
+    apply vcg
+    done
+next
+  case (3 a k x b c s y d)
+  note [vcg_rules] = 3
+  show ?case
+    apply (subst combine.simps)
+    apply vcg
+    subgoal
+      apply resolve_rbt_pat_mat
+      apply vcg
+      unfolding rbt_assn_branch_def
+      apply vcg_try_solve
+      done
+    subgoal
+      apply vcg
+      apply simp
+      apply (cases "rbt_combine b c")
+       apply auto
+      subgoal
+        unfolding rbt_assn_branch_def
+        apply vcg
+        done
+      subgoal for col
+        apply (auto split: color.splits)
+        apply (rule close_rbt_assn[where ti=ri], vcg_solve)
+        apply (rule close_rbt_assn[where ti=li], vcg_solve)
+        apply vcg
+        done
+        (*broken*)
+        (*
+        apply (cases col, auto)
+        unfolding rbt_assn_branch_def
+        apply vcg_solve
+        apply fri_dbg_start
+        apply (rule fri_exE)+
+        apply fri_dbg_step
+
+        apply fri_dbg_step
+         apply fri_dbg_step
+         apply vcg_try_solve
+        apply fri_dbg_step
+        apply fri_dbg_step
+        apply fri_dbg_step
+        apply fri_dbg_step
+        apply fri_dbg_step
+         apply fri_dbg_step
+         apply vcg_try_solve
+        apply fri_dbg_step
+        apply fri_dbg_step
+        sorry
+      *)
+      done
+    done
+next
+  case (4 a k x b c s y d)
+  note [vcg_rules] = 4
+  show ?case
+    apply (subst combine.simps)
+    apply vcg
+    subgoal
+      apply resolve_rbt_pat_mat
+      apply vcg
+      apply (simp add: rbt_assn_branch_def)
+      apply vcg
+      done
+    subgoal
+      apply vcg
+      apply (erule close_rbt_assn, vcg_solve)
+      apply vcg
+      apply (cases "rbt_combine b c")
+      subgoal 
+        apply auto
+        apply vcg
+        done
+      subgoal
+        apply (auto split: color.splits)
+        apply vcg
+        done
+      done
+    done
+next
+  case (5 va vb vc vd b k x c)
+
+  note [vcg_rules] = 5
+
+  show ?case
+    apply (subst combine.simps)
+    apply vcg
+    apply (erule close_rbt_assn[where ti=li], vcg_solve)
+    apply vcg
+    apply (rule close_rbt_assn[where ti=ri], vcg_solve)
+    apply vcg
+    done
+next
+  case (6 a k x b va vb vc vd)
+  note [vcg_rules] = 6
+  show ?case
+    apply (subst combine.simps)
+    apply vcg
+    apply (erule close_rbt_assn[where ti=ri], vcg_solve)
+    apply vcg
+    apply (rule close_rbt_assn[where ti=li], vcg_solve)
+    apply vcg    
+    done
+qed
+
+
 end
+
 
 end
